

# PROOF OF KNUTH BINOMIAL IDENTITY (5.43)

## 1. PRELIMINARIES

**Proposition 1.1** (Falling binomial identity).

$$\binom{n}{k} = \frac{(n)_k}{k!}$$

**Proposition 1.2** (Binomial-Stirling form).

$$\binom{n}{k} = \frac{(n)_k}{k!} = \frac{1}{k!} \sum_{j=0}^k (-1)^j \begin{bmatrix} k \\ j \end{bmatrix} n^j$$

Thus, the explicit form

**Corollary 1.3** (Explicit Binomial-Stirling form).

$$\binom{n}{k} = \frac{1}{k!} \left( \begin{bmatrix} k \\ 0 \end{bmatrix} n^0 - \begin{bmatrix} k \\ 1 \end{bmatrix} n^1 + \begin{bmatrix} k \\ 2 \end{bmatrix} n^2 + \cdots + (-1)^{k-1} \begin{bmatrix} k \\ k-1 \end{bmatrix} n^{k-1} + (-1)^k \begin{bmatrix} k \\ k \end{bmatrix} n^k \right)$$

By changing summation order yields

**Corollary 1.4** (Reversed Binomial-Stirling form).

$$\binom{n}{k} = \frac{1}{k!} \sum_{j=0}^k (-1)^{k-j} \begin{bmatrix} k \\ k-j \end{bmatrix} n^{k-j}$$

**Proposition 1.5** (Binomial theorem).

$$\begin{aligned} (r - sk)^j &= \sum_{t=0}^j (-1)^{j-t} \binom{j}{t} r^j s^t k^{j-t} \\ &= (-1)^j (sk)^j + \sum_{t=1}^j (-1)^{j-t} \binom{j}{t} r^j (sk)^{j-t} \end{aligned}$$

## 2. KNUTH IDENTITY

**Proposition 2.1** (Knuth binomial identity).

$$\sum_{k=0}^n \binom{n}{k} \binom{r-sk}{n} (-1)^k = s^n$$

**Proposition 2.2** (Forward finite differences).

$$\Delta^n f(x) = \sum_{k=0}^n \binom{n}{k} (-1)^{n-k} f(x+k)$$

**Proposition 2.3** (Binomial function).

$$F(x) = \binom{r-sx}{n}$$

**Corollary 2.4** (Forward difference of Binomial function).

$$\Delta^t F(x) = \sum_{k=0}^t \binom{t}{k} (-1)^{n-k} \binom{r-s(x+k)}{n}$$